Proving first simple things.
- New test_mvir/test-specs-verify.mvir with simple prove targets
- Fixing treatment of abort in the translator
- Extending driver to recognize boogie errors. Extending test infra to allow expected boogie diagnosis to be annotated in the source.

language/move-prover/bytecode-to-boogie/src/cli.rs
@@ -17,7 +17,7 @@ use std::sync::atomic::{AtomicBool, Ordering};
 pub const INLINE_PRELUDE: &str = "<inline-prelude>";
 
 /// Default flags passed to boogie. Additional flags will be added to this via the -B option.
-const DEFAULT_BOOGIE_FLAGS: &[&str] = &["-doModSetAnalysis"];
+const DEFAULT_BOOGIE_FLAGS: &[&str] = &["-doModSetAnalysis", "-noinfer"];
 
 /// Atomic used to prevent re-initialization of logging.
 static LOGGER_CONFIGURED: AtomicBool = AtomicBool::new(false);
