language/move-prover/bytecode-to-boogie/tests/goldenfiles/test-arithmetic.bpl
@@ -23,7 +23,10 @@ requires ExistsTxnSenderAccount(m, txn);
 
     var tmp: Value;
     var old_size: int;
+
+    var saved_m: Memory;
     assume !abort_flag;
+    saved_m := m;
 
     // assume arguments are of correct types
     assume is#Integer(arg0);
@@ -37,32 +40,46 @@ requires ExistsTxnSenderAccount(m, txn);
     // bytecode translation starts here
     call tmp := CopyOrMoveValue(GetLocal(m, old_size + 0));
     m := UpdateLocal(m, old_size + 4, tmp);
+    if (abort_flag) { goto Label_Abort; }
 
     call tmp := CopyOrMoveValue(GetLocal(m, old_size + 1));
     m := UpdateLocal(m, old_size + 5, tmp);
+    if (abort_flag) { goto Label_Abort; }
 
     call tmp := Add(GetLocal(m, old_size + 4), GetLocal(m, old_size + 5));
     m := UpdateLocal(m, old_size + 6, tmp);
+    if (abort_flag) { goto Label_Abort; }
 
     call tmp := CopyOrMoveValue(GetLocal(m, old_size + 6));
     m := UpdateLocal(m, old_size + 2, tmp);
+    if (abort_flag) { goto Label_Abort; }
 
     call tmp := LdConst(3);
     m := UpdateLocal(m, old_size + 7, tmp);
+    if (abort_flag) { goto Label_Abort; }
 
     call tmp := CopyOrMoveValue(GetLocal(m, old_size + 7));
     m := UpdateLocal(m, old_size + 3, tmp);
+    if (abort_flag) { goto Label_Abort; }
 
     call tmp := CopyOrMoveValue(GetLocal(m, old_size + 3));
     m := UpdateLocal(m, old_size + 8, tmp);
+    if (abort_flag) { goto Label_Abort; }
 
     call tmp := CopyOrMoveValue(GetLocal(m, old_size + 2));
     m := UpdateLocal(m, old_size + 9, tmp);
+    if (abort_flag) { goto Label_Abort; }
 
     ret0 := GetLocal(m, old_size + 8);
     ret1 := GetLocal(m, old_size + 9);
     return;
+    if (abort_flag) { goto Label_Abort; }
 
+Label_Abort:
+    abort_flag := true;
+    m := saved_m;
+    ret0 := DefaultValue;
+    ret1 := DefaultValue;
 }
 
 procedure TestArithmetic_add_two_number_verify (arg0: Value, arg1: Value) returns (ret0: Value, ret1: Value)
@@ -87,7 +104,10 @@ requires ExistsTxnSenderAccount(m, txn);
 
     var tmp: Value;
     var old_size: int;
+
+    var saved_m: Memory;
     assume !abort_flag;
+    saved_m := m;
 
     // assume arguments are of correct types
     assume is#Integer(arg0);
@@ -103,28 +123,40 @@ requires ExistsTxnSenderAccount(m, txn);
     // bytecode translation starts here
     call tmp := CopyOrMoveValue(GetLocal(m, old_size + 0));
     m := UpdateLocal(m, old_size + 4, tmp);
+    if (abort_flag) { goto Label_Abort; }
 
     call tmp := CopyOrMoveValue(GetLocal(m, old_size + 1));
     m := UpdateLocal(m, old_size + 5, tmp);
+    if (abort_flag) { goto Label_Abort; }
 
     call tmp := Add(GetLocal(m, old_size + 4), GetLocal(m, old_size + 5));
     m := UpdateLocal(m, old_size + 6, tmp);
+    if (abort_flag) { goto Label_Abort; }
 
     call tmp := CopyOrMoveValue(GetLocal(m, old_size + 2));
     m := UpdateLocal(m, old_size + 7, tmp);
+    if (abort_flag) { goto Label_Abort; }
 
     call tmp := Mul(GetLocal(m, old_size + 6), GetLocal(m, old_size + 7));
     m := UpdateLocal(m, old_size + 8, tmp);
+    if (abort_flag) { goto Label_Abort; }
 
     call tmp := CopyOrMoveValue(GetLocal(m, old_size + 8));
     m := UpdateLocal(m, old_size + 3, tmp);
+    if (abort_flag) { goto Label_Abort; }
 
     call tmp := CopyOrMoveValue(GetLocal(m, old_size + 3));
     m := UpdateLocal(m, old_size + 9, tmp);
+    if (abort_flag) { goto Label_Abort; }
 
     ret0 := GetLocal(m, old_size + 9);
     return;
+    if (abort_flag) { goto Label_Abort; }
 
+Label_Abort:
+    abort_flag := true;
+    m := saved_m;
+    ret0 := DefaultValue;
 }
 
 procedure TestArithmetic_multiple_ops_verify (arg0: Value, arg1: Value, arg2: Value) returns (ret0: Value)
@@ -162,7 +194,10 @@ requires ExistsTxnSenderAccount(m, txn);
 
     var tmp: Value;
     var old_size: int;
+
+    var saved_m: Memory;
     assume !abort_flag;
+    saved_m := m;
 
     // assume arguments are of correct types
     assume is#Integer(arg0);
@@ -176,75 +211,102 @@ requires ExistsTxnSenderAccount(m, txn);
     // bytecode translation starts here
     call tmp := CopyOrMoveValue(GetLocal(m, old_size + 0));
     m := UpdateLocal(m, old_size + 4, tmp);
+    if (abort_flag) { goto Label_Abort; }
 
     call tmp := CopyOrMoveValue(GetLocal(m, old_size + 1));
     m := UpdateLocal(m, old_size + 5, tmp);
+    if (abort_flag) { goto Label_Abort; }
 
     call tmp := Gt(GetLocal(m, old_size + 4), GetLocal(m, old_size + 5));
     m := UpdateLocal(m, old_size + 6, tmp);
+    if (abort_flag) { goto Label_Abort; }
 
     call tmp := CopyOrMoveValue(GetLocal(m, old_size + 0));
     m := UpdateLocal(m, old_size + 7, tmp);
+    if (abort_flag) { goto Label_Abort; }
 
     call tmp := CopyOrMoveValue(GetLocal(m, old_size + 1));
     m := UpdateLocal(m, old_size + 8, tmp);
+    if (abort_flag) { goto Label_Abort; }
 
     call tmp := Ge(GetLocal(m, old_size + 7), GetLocal(m, old_size + 8));
     m := UpdateLocal(m, old_size + 9, tmp);
+    if (abort_flag) { goto Label_Abort; }
 
     call tmp := And(GetLocal(m, old_size + 6), GetLocal(m, old_size + 9));
     m := UpdateLocal(m, old_size + 10, tmp);
+    if (abort_flag) { goto Label_Abort; }
 
     call tmp := CopyOrMoveValue(GetLocal(m, old_size + 10));
     m := UpdateLocal(m, old_size + 2, tmp);
+    if (abort_flag) { goto Label_Abort; }
 
     call tmp := CopyOrMoveValue(GetLocal(m, old_size + 0));
     m := UpdateLocal(m, old_size + 11, tmp);
+    if (abort_flag) { goto Label_Abort; }
 
     call tmp := CopyOrMoveValue(GetLocal(m, old_size + 1));
     m := UpdateLocal(m, old_size + 12, tmp);
+    if (abort_flag) { goto Label_Abort; }
 
     call tmp := Lt(GetLocal(m, old_size + 11), GetLocal(m, old_size + 12));
     m := UpdateLocal(m, old_size + 13, tmp);
+    if (abort_flag) { goto Label_Abort; }
 
     call tmp := CopyOrMoveValue(GetLocal(m, old_size + 0));
     m := UpdateLocal(m, old_size + 14, tmp);
+    if (abort_flag) { goto Label_Abort; }
 
     call tmp := CopyOrMoveValue(GetLocal(m, old_size + 1));
     m := UpdateLocal(m, old_size + 15, tmp);
+    if (abort_flag) { goto Label_Abort; }
 
     call tmp := Le(GetLocal(m, old_size + 14), GetLocal(m, old_size + 15));
     m := UpdateLocal(m, old_size + 16, tmp);
+    if (abort_flag) { goto Label_Abort; }
 
     call tmp := Or(GetLocal(m, old_size + 13), GetLocal(m, old_size + 16));
     m := UpdateLocal(m, old_size + 17, tmp);
+    if (abort_flag) { goto Label_Abort; }
 
     call tmp := CopyOrMoveValue(GetLocal(m, old_size + 17));
     m := UpdateLocal(m, old_size + 3, tmp);
+    if (abort_flag) { goto Label_Abort; }
 
     call tmp := CopyOrMoveValue(GetLocal(m, old_size + 2));
     m := UpdateLocal(m, old_size + 18, tmp);
+    if (abort_flag) { goto Label_Abort; }
 
     call tmp := CopyOrMoveValue(GetLocal(m, old_size + 3));
     m := UpdateLocal(m, old_size + 19, tmp);
+    if (abort_flag) { goto Label_Abort; }
 
     tmp := Boolean(!IsEqual(GetLocal(m, old_size + 18), GetLocal(m, old_size + 19)));
     m := UpdateLocal(m, old_size + 20, tmp);
+    if (abort_flag) { goto Label_Abort; }
 
     call tmp := Not(GetLocal(m, old_size + 20));
     m := UpdateLocal(m, old_size + 21, tmp);
+    if (abort_flag) { goto Label_Abort; }
 
     tmp := GetLocal(m, old_size + 21);
     if (!b#Boolean(tmp)) { goto Label_23; }
+    if (abort_flag) { goto Label_Abort; }
 
     call tmp := LdConst(42);
     m := UpdateLocal(m, old_size + 22, tmp);
+    if (abort_flag) { goto Label_Abort; }
 
-    assert false;
+    goto Label_Abort;
+    if (abort_flag) { goto Label_Abort; }
 
 Label_23:
     return;
+    if (abort_flag) { goto Label_Abort; }
 
+Label_Abort:
+    abort_flag := true;
+    m := saved_m;
 }
 
 procedure TestArithmetic_bool_ops_verify (arg0: Value, arg1: Value) returns ()
@@ -280,7 +342,10 @@ requires ExistsTxnSenderAccount(m, txn);
 
     var tmp: Value;
     var old_size: int;
+
+    var saved_m: Memory;
     assume !abort_flag;
+    saved_m := m;
 
     // assume arguments are of correct types
     assume is#Integer(arg0);
@@ -294,71 +359,98 @@ requires ExistsTxnSenderAccount(m, txn);
     // bytecode translation starts here
     call tmp := LdConst(6);
     m := UpdateLocal(m, old_size + 3, tmp);
+    if (abort_flag) { goto Label_Abort; }
 
     call tmp := LdConst(4);
     m := UpdateLocal(m, old_size + 4, tmp);
+    if (abort_flag) { goto Label_Abort; }
 
     call tmp := Add(GetLocal(m, old_size + 3), GetLocal(m, old_size + 4));
     m := UpdateLocal(m, old_size + 5, tmp);
+    if (abort_flag) { goto Label_Abort; }
 
     call tmp := LdConst(1);
     m := UpdateLocal(m, old_size + 6, tmp);
+    if (abort_flag) { goto Label_Abort; }
 
     call tmp := Sub(GetLocal(m, old_size + 5), GetLocal(m, old_size + 6));
     m := UpdateLocal(m, old_size + 7, tmp);
+    if (abort_flag) { goto Label_Abort; }
 
     call tmp := LdConst(2);
     m := UpdateLocal(m, old_size + 8, tmp);
+    if (abort_flag) { goto Label_Abort; }
 
     call tmp := Mul(GetLocal(m, old_size + 7), GetLocal(m, old_size + 8));
     m := UpdateLocal(m, old_size + 9, tmp);
+    if (abort_flag) { goto Label_Abort; }
 
     call tmp := LdConst(3);
     m := UpdateLocal(m, old_size + 10, tmp);
+    if (abort_flag) { goto Label_Abort; }
 
     call tmp := Div(GetLocal(m, old_size + 9), GetLocal(m, old_size + 10));
     m := UpdateLocal(m, old_size + 11, tmp);
+    if (abort_flag) { goto Label_Abort; }
 
     call tmp := LdConst(4);
     m := UpdateLocal(m, old_size + 12, tmp);
+    if (abort_flag) { goto Label_Abort; }
 
     call tmp := Mod(GetLocal(m, old_size + 11), GetLocal(m, old_size + 12));
     m := UpdateLocal(m, old_size + 13, tmp);
+    if (abort_flag) { goto Label_Abort; }
 
     call tmp := CopyOrMoveValue(GetLocal(m, old_size + 13));
     m := UpdateLocal(m, old_size + 2, tmp);
+    if (abort_flag) { goto Label_Abort; }
 
     call tmp := CopyOrMoveValue(GetLocal(m, old_size + 2));
     m := UpdateLocal(m, old_size + 14, tmp);
+    if (abort_flag) { goto Label_Abort; }
 
     call tmp := LdConst(2);
     m := UpdateLocal(m, old_size + 15, tmp);
+    if (abort_flag) { goto Label_Abort; }
 
     tmp := Boolean(IsEqual(GetLocal(m, old_size + 14), GetLocal(m, old_size + 15)));
     m := UpdateLocal(m, old_size + 16, tmp);
+    if (abort_flag) { goto Label_Abort; }
 
     call tmp := Not(GetLocal(m, old_size + 16));
     m := UpdateLocal(m, old_size + 17, tmp);
+    if (abort_flag) { goto Label_Abort; }
 
     tmp := GetLocal(m, old_size + 17);
     if (!b#Boolean(tmp)) { goto Label_19; }
+    if (abort_flag) { goto Label_Abort; }
 
     call tmp := LdConst(42);
     m := UpdateLocal(m, old_size + 18, tmp);
+    if (abort_flag) { goto Label_Abort; }
 
-    assert false;
+    goto Label_Abort;
+    if (abort_flag) { goto Label_Abort; }
 
 Label_19:
     call tmp := CopyOrMoveValue(GetLocal(m, old_size + 2));
     m := UpdateLocal(m, old_size + 19, tmp);
+    if (abort_flag) { goto Label_Abort; }
 
     call tmp := CopyOrMoveValue(GetLocal(m, old_size + 0));
     m := UpdateLocal(m, old_size + 20, tmp);
+    if (abort_flag) { goto Label_Abort; }
 
     ret0 := GetLocal(m, old_size + 19);
     ret1 := GetLocal(m, old_size + 20);
     return;
+    if (abort_flag) { goto Label_Abort; }
 
+Label_Abort:
+    abort_flag := true;
+    m := saved_m;
+    ret0 := DefaultValue;
+    ret1 := DefaultValue;
 }
 
 procedure TestArithmetic_arithmetic_ops_verify (arg0: Value, arg1: Value) returns (ret0: Value, ret1: Value)
@@ -379,7 +471,10 @@ requires ExistsTxnSenderAccount(m, txn);
 
     var tmp: Value;
     var old_size: int;
+
+    var saved_m: Memory;
     assume !abort_flag;
+    saved_m := m;
 
     // assume arguments are of correct types
 
@@ -389,24 +484,34 @@ requires ExistsTxnSenderAccount(m, txn);
     // bytecode translation starts here
     call tmp := LdConst(9223372036854775807);
     m := UpdateLocal(m, old_size + 2, tmp);
+    if (abort_flag) { goto Label_Abort; }
 
     call tmp := CopyOrMoveValue(GetLocal(m, old_size + 2));
     m := UpdateLocal(m, old_size + 0, tmp);
+    if (abort_flag) { goto Label_Abort; }
 
     call tmp := CopyOrMoveValue(GetLocal(m, old_size + 0));
     m := UpdateLocal(m, old_size + 3, tmp);
+    if (abort_flag) { goto Label_Abort; }
 
     call tmp := LdConst(1);
     m := UpdateLocal(m, old_size + 4, tmp);
+    if (abort_flag) { goto Label_Abort; }
 
     call tmp := Add(GetLocal(m, old_size + 3), GetLocal(m, old_size + 4));
     m := UpdateLocal(m, old_size + 5, tmp);
+    if (abort_flag) { goto Label_Abort; }
 
     call tmp := CopyOrMoveValue(GetLocal(m, old_size + 5));
     m := UpdateLocal(m, old_size + 1, tmp);
+    if (abort_flag) { goto Label_Abort; }
 
     return;
+    if (abort_flag) { goto Label_Abort; }
 
+Label_Abort:
+    abort_flag := true;
+    m := saved_m;
 }
 
 procedure TestArithmetic_overflow_verify () returns ()
@@ -427,7 +532,10 @@ requires ExistsTxnSenderAccount(m, txn);
 
     var tmp: Value;
     var old_size: int;
+
+    var saved_m: Memory;
     assume !abort_flag;
+    saved_m := m;
 
     // assume arguments are of correct types
 
@@ -437,24 +545,34 @@ requires ExistsTxnSenderAccount(m, txn);
     // bytecode translation starts here
     call tmp := LdConst(0);
     m := UpdateLocal(m, old_size + 2, tmp);
+    if (abort_flag) { goto Label_Abort; }
 
     call tmp := CopyOrMoveValue(GetLocal(m, old_size + 2));
     m := UpdateLocal(m, old_size + 0, tmp);
+    if (abort_flag) { goto Label_Abort; }
 
     call tmp := CopyOrMoveValue(GetLocal(m, old_size + 0));
     m := UpdateLocal(m, old_size + 3, tmp);
+    if (abort_flag) { goto Label_Abort; }
 
     call tmp := LdConst(1);
     m := UpdateLocal(m, old_size + 4, tmp);
+    if (abort_flag) { goto Label_Abort; }
 
     call tmp := Sub(GetLocal(m, old_size + 3), GetLocal(m, old_size + 4));
     m := UpdateLocal(m, old_size + 5, tmp);
+    if (abort_flag) { goto Label_Abort; }
 
     call tmp := CopyOrMoveValue(GetLocal(m, old_size + 5));
     m := UpdateLocal(m, old_size + 1, tmp);
+    if (abort_flag) { goto Label_Abort; }
 
     return;
+    if (abort_flag) { goto Label_Abort; }
 
+Label_Abort:
+    abort_flag := true;
+    m := saved_m;
 }
 
 procedure TestArithmetic_underflow_verify () returns ()
@@ -475,7 +593,10 @@ requires ExistsTxnSenderAccount(m, txn);
 
     var tmp: Value;
     var old_size: int;
+
+    var saved_m: Memory;
     assume !abort_flag;
+    saved_m := m;
 
     // assume arguments are of correct types
 
@@ -485,24 +606,34 @@ requires ExistsTxnSenderAccount(m, txn);
     // bytecode translation starts here
     call tmp := LdConst(0);
     m := UpdateLocal(m, old_size + 2, tmp);
+    if (abort_flag) { goto Label_Abort; }
 
     call tmp := CopyOrMoveValue(GetLocal(m, old_size + 2));
     m := UpdateLocal(m, old_size + 0, tmp);
+    if (abort_flag) { goto Label_Abort; }
 
     call tmp := LdConst(1);
     m := UpdateLocal(m, old_size + 3, tmp);
+    if (abort_flag) { goto Label_Abort; }
 
     call tmp := CopyOrMoveValue(GetLocal(m, old_size + 0));
     m := UpdateLocal(m, old_size + 4, tmp);
+    if (abort_flag) { goto Label_Abort; }
 
     call tmp := Div(GetLocal(m, old_size + 3), GetLocal(m, old_size + 4));
     m := UpdateLocal(m, old_size + 5, tmp);
+    if (abort_flag) { goto Label_Abort; }
 
     call tmp := CopyOrMoveValue(GetLocal(m, old_size + 5));
     m := UpdateLocal(m, old_size + 1, tmp);
+    if (abort_flag) { goto Label_Abort; }
 
     return;
+    if (abort_flag) { goto Label_Abort; }
 
+Label_Abort:
+    abort_flag := true;
+    m := saved_m;
 }
 
 procedure TestArithmetic_div_by_zero_verify () returns ()
