language/move-prover/bytecode-to-boogie/tests/goldenfiles/test-control-flow.bpl
@@ -19,7 +19,10 @@ requires ExistsTxnSenderAccount(m, txn);
 
     var tmp: Value;
     var old_size: int;
+
+    var saved_m: Memory;
     assume !abort_flag;
+    saved_m := m;
 
     // assume arguments are of correct types
     assume is#Boolean(arg0);
@@ -31,29 +34,41 @@ requires ExistsTxnSenderAccount(m, txn);
     // bytecode translation starts here
     call tmp := CopyOrMoveValue(GetLocal(m, old_size + 0));
     m := UpdateLocal(m, old_size + 1, tmp);
+    if (abort_flag) { goto Label_Abort; }
 
     tmp := GetLocal(m, old_size + 1);
     if (!b#Boolean(tmp)) { goto Label_6; }
+    if (abort_flag) { goto Label_Abort; }
 
     call tmp := LdConst(1);
     m := UpdateLocal(m, old_size + 2, tmp);
+    if (abort_flag) { goto Label_Abort; }
 
     call tmp := LdConst(2);
     m := UpdateLocal(m, old_size + 3, tmp);
+    if (abort_flag) { goto Label_Abort; }
 
     call tmp := Add(GetLocal(m, old_size + 2), GetLocal(m, old_size + 3));
     m := UpdateLocal(m, old_size + 4, tmp);
+    if (abort_flag) { goto Label_Abort; }
 
     ret0 := GetLocal(m, old_size + 4);
     return;
+    if (abort_flag) { goto Label_Abort; }
 
 Label_6:
     call tmp := LdConst(0);
     m := UpdateLocal(m, old_size + 5, tmp);
+    if (abort_flag) { goto Label_Abort; }
 
     ret0 := GetLocal(m, old_size + 5);
     return;
+    if (abort_flag) { goto Label_Abort; }
 
+Label_Abort:
+    abort_flag := true;
+    m := saved_m;
+    ret0 := DefaultValue;
 }
 
 procedure TestControlFlow_branch_once_verify (arg0: Value) returns (ret0: Value)
