language/move-prover/bytecode-to-boogie/tests/goldenfiles/test-generics.bpl
@@ -65,7 +65,10 @@ requires ExistsTxnSenderAccount(m, txn);
 
     var tmp: Value;
     var old_size: int;
+
+    var saved_m: Memory;
     assume !abort_flag;
+    saved_m := m;
 
     // assume arguments are of correct types
     assume is#Integer(arg0);
@@ -81,42 +84,59 @@ requires ExistsTxnSenderAccount(m, txn);
     assume is#Vector(t4);
 
     m := UpdateLocal(m, old_size + 4, t4);
+    if (abort_flag) { goto Label_Abort; }
 
     call tmp := CopyOrMoveValue(GetLocal(m, old_size + 4));
     m := UpdateLocal(m, old_size + 2, tmp);
+    if (abort_flag) { goto Label_Abort; }
 
     call t5 := BorrowLoc(old_size+2);
+    if (abort_flag) { goto Label_Abort; }
 
     call tmp := CopyOrMoveValue(GetLocal(m, old_size + 0));
     m := UpdateLocal(m, old_size + 6, tmp);
+    if (abort_flag) { goto Label_Abort; }
 
     call Vector_push_back(IntegerType(), t5, GetLocal(m, old_size + 6));
+    if (abort_flag) { goto Label_Abort; }
 
     call t7 := BorrowLoc(old_size+2);
+    if (abort_flag) { goto Label_Abort; }
 
     call tmp := CopyOrMoveValue(GetLocal(m, old_size + 1));
     m := UpdateLocal(m, old_size + 8, tmp);
+    if (abort_flag) { goto Label_Abort; }
 
     call Vector_push_back(IntegerType(), t7, GetLocal(m, old_size + 8));
+    if (abort_flag) { goto Label_Abort; }
 
     call tmp := CopyOrMoveValue(GetLocal(m, old_size + 2));
     m := UpdateLocal(m, old_size + 9, tmp);
+    if (abort_flag) { goto Label_Abort; }
 
     assume is#Vector(GetLocal(m, old_size + 9));
 
     call tmp := Pack_TestGenerics_R(GetLocal(m, old_size + 9));
     m := UpdateLocal(m, old_size + 10, tmp);
+    if (abort_flag) { goto Label_Abort; }
 
     call tmp := CopyOrMoveValue(GetLocal(m, old_size + 10));
     m := UpdateLocal(m, old_size + 3, tmp);
+    if (abort_flag) { goto Label_Abort; }
 
     call tmp := CopyOrMoveValue(GetLocal(m, old_size + 3));
     m := UpdateLocal(m, old_size + 11, tmp);
+    if (abort_flag) { goto Label_Abort; }
 
     call MoveToSender(TestGenerics_R_type_value(), GetLocal(m, old_size + 11));
+    if (abort_flag) { goto Label_Abort; }
 
     return;
+    if (abort_flag) { goto Label_Abort; }
 
+Label_Abort:
+    abort_flag := true;
+    m := saved_m;
 }
 
 procedure TestGenerics_move2_verify (arg0: Value, arg1: Value) returns ()
@@ -138,7 +158,10 @@ requires ExistsTxnSenderAccount(m, txn);
 
     var tmp: Value;
     var old_size: int;
+
+    var saved_m: Memory;
     assume !abort_flag;
+    saved_m := m;
 
     // assume arguments are of correct types
 
@@ -151,28 +174,40 @@ requires ExistsTxnSenderAccount(m, txn);
     assume is#Vector(t2);
 
     m := UpdateLocal(m, old_size + 2, t2);
+    if (abort_flag) { goto Label_Abort; }
 
     call tmp := CopyOrMoveValue(GetLocal(m, old_size + 2));
     m := UpdateLocal(m, old_size + 1, tmp);
+    if (abort_flag) { goto Label_Abort; }
 
     call t3 := BorrowLoc(old_size+1);
+    if (abort_flag) { goto Label_Abort; }
 
     call tmp := CopyOrMoveValue(GetLocal(m, old_size + 0));
     m := UpdateLocal(m, old_size + 4, tmp);
+    if (abort_flag) { goto Label_Abort; }
 
     call Vector_push_back(tv0, t3, GetLocal(m, old_size + 4));
+    if (abort_flag) { goto Label_Abort; }
 
     call tmp := CopyOrMoveValue(GetLocal(m, old_size + 1));
     m := UpdateLocal(m, old_size + 5, tmp);
+    if (abort_flag) { goto Label_Abort; }
 
     assume is#Vector(GetLocal(m, old_size + 5));
 
     call tmp := Pack_TestGenerics_T(tv0, GetLocal(m, old_size + 5));
     m := UpdateLocal(m, old_size + 6, tmp);
+    if (abort_flag) { goto Label_Abort; }
 
     ret0 := GetLocal(m, old_size + 6);
     return;
+    if (abort_flag) { goto Label_Abort; }
 
+Label_Abort:
+    abort_flag := true;
+    m := saved_m;
+    ret0 := DefaultValue;
 }
 
 procedure TestGenerics_create_verify (tv0: TypeValue, arg0: Value) returns (ret0: Value)
@@ -200,7 +235,10 @@ requires ExistsTxnSenderAccount(m, txn);
 
     var tmp: Value;
     var old_size: int;
+
+    var saved_m: Memory;
     assume !abort_flag;
+    saved_m := m;
 
     // assume arguments are of correct types
 
@@ -212,44 +250,60 @@ requires ExistsTxnSenderAccount(m, txn);
     // bytecode translation starts here
     call tmp := CopyOrMoveValue(GetLocal(m, old_size + 0));
     m := UpdateLocal(m, old_size + 5, tmp);
+    if (abort_flag) { goto Label_Abort; }
 
     call t6 := TestGenerics_create(tv0, GetLocal(m, old_size + 5));
     assume is#Vector(t6);
 
     m := UpdateLocal(m, old_size + 6, t6);
+    if (abort_flag) { goto Label_Abort; }
 
     call tmp := CopyOrMoveValue(GetLocal(m, old_size + 6));
     m := UpdateLocal(m, old_size + 3, tmp);
+    if (abort_flag) { goto Label_Abort; }
 
     call tmp := CopyOrMoveValue(GetLocal(m, old_size + 1));
     m := UpdateLocal(m, old_size + 7, tmp);
+    if (abort_flag) { goto Label_Abort; }
 
     call t8 := TestGenerics_create(tv0, GetLocal(m, old_size + 7));
     assume is#Vector(t8);
 
     m := UpdateLocal(m, old_size + 8, t8);
+    if (abort_flag) { goto Label_Abort; }
 
     call tmp := CopyOrMoveValue(GetLocal(m, old_size + 8));
     m := UpdateLocal(m, old_size + 4, tmp);
+    if (abort_flag) { goto Label_Abort; }
 
     call tmp := CopyOrMoveValue(GetLocal(m, old_size + 3));
     m := UpdateLocal(m, old_size + 9, tmp);
+    if (abort_flag) { goto Label_Abort; }
 
     call tmp := CopyOrMoveValue(GetLocal(m, old_size + 4));
     m := UpdateLocal(m, old_size + 10, tmp);
+    if (abort_flag) { goto Label_Abort; }
 
     tmp := Boolean(IsEqual(GetLocal(m, old_size + 9), GetLocal(m, old_size + 10)));
     m := UpdateLocal(m, old_size + 11, tmp);
+    if (abort_flag) { goto Label_Abort; }
 
     call tmp := CopyOrMoveValue(GetLocal(m, old_size + 11));
     m := UpdateLocal(m, old_size + 2, tmp);
+    if (abort_flag) { goto Label_Abort; }
 
     call tmp := CopyOrMoveValue(GetLocal(m, old_size + 2));
     m := UpdateLocal(m, old_size + 12, tmp);
+    if (abort_flag) { goto Label_Abort; }
 
     ret0 := GetLocal(m, old_size + 12);
     return;
+    if (abort_flag) { goto Label_Abort; }
 
+Label_Abort:
+    abort_flag := true;
+    m := saved_m;
+    ret0 := DefaultValue;
 }
 
 procedure TestGenerics_overcomplicated_equals_verify (tv0: TypeValue, arg0: Value, arg1: Value) returns (ret0: Value)
@@ -269,7 +323,10 @@ requires ExistsTxnSenderAccount(m, txn);
 
     var tmp: Value;
     var old_size: int;
+
+    var saved_m: Memory;
     assume !abort_flag;
+    saved_m := m;
 
     // assume arguments are of correct types
 
@@ -279,24 +336,34 @@ requires ExistsTxnSenderAccount(m, txn);
     // bytecode translation starts here
     call tmp := LdConst(1);
     m := UpdateLocal(m, old_size + 1, tmp);
+    if (abort_flag) { goto Label_Abort; }
 
     call tmp := LdConst(1);
     m := UpdateLocal(m, old_size + 2, tmp);
+    if (abort_flag) { goto Label_Abort; }
 
     call t3 := TestGenerics_overcomplicated_equals(IntegerType(), GetLocal(m, old_size + 1), GetLocal(m, old_size + 2));
     assume is#Boolean(t3);
 
     m := UpdateLocal(m, old_size + 3, t3);
+    if (abort_flag) { goto Label_Abort; }
 
     call tmp := CopyOrMoveValue(GetLocal(m, old_size + 3));
     m := UpdateLocal(m, old_size + 0, tmp);
+    if (abort_flag) { goto Label_Abort; }
 
     call tmp := CopyOrMoveValue(GetLocal(m, old_size + 0));
     m := UpdateLocal(m, old_size + 4, tmp);
+    if (abort_flag) { goto Label_Abort; }
 
     ret0 := GetLocal(m, old_size + 4);
     return;
+    if (abort_flag) { goto Label_Abort; }
 
+Label_Abort:
+    abort_flag := true;
+    m := saved_m;
+    ret0 := DefaultValue;
 }
 
 procedure TestGenerics_test_verify () returns (ret0: Value)
