language/move-prover/bytecode-to-boogie/tests/goldenfiles/test-specs-verify.bpl
@@ -1,0 +1,301 @@
+
+
+// ** structs of module TestSpecs
+
+const unique TestSpecs_R: TypeName;
+const TestSpecs_R_x: FieldName;
+axiom TestSpecs_R_x == 0;
+function TestSpecs_R_type_value(): TypeValue {
+    StructType(TestSpecs_R, ExtendTypeValueArray(EmptyTypeValueArray, IntegerType()))
+}
+
+procedure {:inline 1} Pack_TestSpecs_R(v0: Value) returns (v: Value)
+{
+    assume is#Integer(v0);
+    v := Vector(ExtendValueArray(EmptyValueArray, v0));
+
+}
+
+procedure {:inline 1} Unpack_TestSpecs_R(v: Value) returns (v0: Value)
+{
+    assume is#Vector(v);
+    v0 := SelectField(v, TestSpecs_R_x);
+}
+
+
+
+// ** functions of module TestSpecs
+
+procedure {:inline 1} TestSpecs_create_resource () returns ()
+requires ExistsTxnSenderAccount(m, txn);
+ensures !abort_flag ==> b#Boolean(ExistsResource(m, TestSpecs_R_type_value(), a#Address(Address(TxnSenderAddress(txn)))));
+ensures !(b#Boolean(ExistsResource(m, TestSpecs_R_type_value(), a#Address(Address(TxnSenderAddress(txn)))))) ==> !abort_flag;
+{
+    // declare local variables
+    var t0: Value; // AddressType()
+    var t1: Value; // BooleanType()
+    var t2: Value; // IntegerType()
+    var t3: Value; // IntegerType()
+    var t4: Value; // TestSpecs_R_type_value()
+
+    var tmp: Value;
+    var old_size: int;
+
+    var saved_m: Memory;
+    assume !abort_flag;
+    saved_m := m;
+
+    // assume arguments are of correct types
+
+    old_size := local_counter;
+    local_counter := local_counter + 5;
+
+    // bytecode translation starts here
+    call tmp := GetTxnSenderAddress();
+    m := UpdateLocal(m, old_size + 0, tmp);
+    if (abort_flag) { goto Label_Abort; }
+
+    call tmp := Exists(GetLocal(m, old_size + 0), TestSpecs_R_type_value());
+    m := UpdateLocal(m, old_size + 1, tmp);
+    if (abort_flag) { goto Label_Abort; }
+
+    tmp := GetLocal(m, old_size + 1);
+    if (!b#Boolean(tmp)) { goto Label_5; }
+    if (abort_flag) { goto Label_Abort; }
+
+    call tmp := LdConst(1);
+    m := UpdateLocal(m, old_size + 2, tmp);
+    if (abort_flag) { goto Label_Abort; }
+
+    goto Label_Abort;
+    if (abort_flag) { goto Label_Abort; }
+
+Label_5:
+    call tmp := LdConst(1);
+    m := UpdateLocal(m, old_size + 3, tmp);
+    if (abort_flag) { goto Label_Abort; }
+
+    assume is#Integer(GetLocal(m, old_size + 3));
+
+    call tmp := Pack_TestSpecs_R(GetLocal(m, old_size + 3));
+    m := UpdateLocal(m, old_size + 4, tmp);
+    if (abort_flag) { goto Label_Abort; }
+
+    call MoveToSender(TestSpecs_R_type_value(), GetLocal(m, old_size + 4));
+    if (abort_flag) { goto Label_Abort; }
+
+    return;
+    if (abort_flag) { goto Label_Abort; }
+
+Label_Abort:
+    abort_flag := true;
+    m := saved_m;
+}
+
+procedure TestSpecs_create_resource_verify () returns ()
+{
+    call TestSpecs_create_resource();
+}
+
+procedure {:inline 1} TestSpecs_create_resource_error () returns ()
+requires ExistsTxnSenderAccount(m, txn);
+ensures !abort_flag ==> b#Boolean(ExistsResource(m, TestSpecs_R_type_value(), a#Address(Address(TxnSenderAddress(txn)))));
+ensures !(b#Boolean(ExistsResource(m, TestSpecs_R_type_value(), a#Address(Address(TxnSenderAddress(txn)))))) ==> !abort_flag;
+{
+    // declare local variables
+    var t0: Value; // AddressType()
+    var t1: Value; // BooleanType()
+    var t2: Value; // IntegerType()
+    var t3: Value; // IntegerType()
+    var t4: Value; // TestSpecs_R_type_value()
+
+    var tmp: Value;
+    var old_size: int;
+
+    var saved_m: Memory;
+    assume !abort_flag;
+    saved_m := m;
+
+    // assume arguments are of correct types
+
+    old_size := local_counter;
+    local_counter := local_counter + 5;
+
+    // bytecode translation starts here
+    call tmp := GetTxnSenderAddress();
+    m := UpdateLocal(m, old_size + 0, tmp);
+    if (abort_flag) { goto Label_Abort; }
+
+    call tmp := Exists(GetLocal(m, old_size + 0), TestSpecs_R_type_value());
+    m := UpdateLocal(m, old_size + 1, tmp);
+    if (abort_flag) { goto Label_Abort; }
+
+    tmp := GetLocal(m, old_size + 1);
+    if (!b#Boolean(tmp)) { goto Label_5; }
+    if (abort_flag) { goto Label_Abort; }
+
+    call tmp := LdConst(1);
+    m := UpdateLocal(m, old_size + 2, tmp);
+    if (abort_flag) { goto Label_Abort; }
+
+    goto Label_Abort;
+    if (abort_flag) { goto Label_Abort; }
+
+Label_5:
+    call tmp := LdConst(1);
+    m := UpdateLocal(m, old_size + 3, tmp);
+    if (abort_flag) { goto Label_Abort; }
+
+    assume is#Integer(GetLocal(m, old_size + 3));
+
+    call tmp := Pack_TestSpecs_R(GetLocal(m, old_size + 3));
+    m := UpdateLocal(m, old_size + 4, tmp);
+    if (abort_flag) { goto Label_Abort; }
+
+    call MoveToSender(TestSpecs_R_type_value(), GetLocal(m, old_size + 4));
+    if (abort_flag) { goto Label_Abort; }
+
+    return;
+    if (abort_flag) { goto Label_Abort; }
+
+Label_Abort:
+    abort_flag := true;
+    m := saved_m;
+}
+
+procedure TestSpecs_create_resource_error_verify () returns ()
+{
+    call TestSpecs_create_resource_error();
+}
+
+procedure {:inline 1} TestSpecs_div_by_zero (arg0: Value, arg1: Value) returns (ret0: Value)
+requires ExistsTxnSenderAccount(m, txn);
+ensures !old(b#Boolean(Boolean(i#Integer(arg1) > i#Integer(Integer(0))))) ==> abort_flag;
+ensures (b#Boolean(Boolean(i#Integer(arg1) > i#Integer(Integer(0))))) ==> !abort_flag;
+{
+    // declare local variables
+    var t0: Value; // IntegerType()
+    var t1: Value; // IntegerType()
+    var t2: Value; // IntegerType()
+    var t3: Value; // IntegerType()
+    var t4: Value; // IntegerType()
+    var t5: Value; // IntegerType()
+    var t6: Value; // IntegerType()
+
+    var tmp: Value;
+    var old_size: int;
+
+    var saved_m: Memory;
+    assume !abort_flag;
+    saved_m := m;
+
+    // assume arguments are of correct types
+    assume is#Integer(arg0);
+    assume is#Integer(arg1);
+
+    old_size := local_counter;
+    local_counter := local_counter + 7;
+    m := UpdateLocal(m, old_size + 0, arg0);
+    m := UpdateLocal(m, old_size + 1, arg1);
+
+    // bytecode translation starts here
+    call tmp := CopyOrMoveValue(GetLocal(m, old_size + 0));
+    m := UpdateLocal(m, old_size + 3, tmp);
+    if (abort_flag) { goto Label_Abort; }
+
+    call tmp := CopyOrMoveValue(GetLocal(m, old_size + 1));
+    m := UpdateLocal(m, old_size + 4, tmp);
+    if (abort_flag) { goto Label_Abort; }
+
+    call tmp := Div(GetLocal(m, old_size + 3), GetLocal(m, old_size + 4));
+    m := UpdateLocal(m, old_size + 5, tmp);
+    if (abort_flag) { goto Label_Abort; }
+
+    call tmp := CopyOrMoveValue(GetLocal(m, old_size + 5));
+    m := UpdateLocal(m, old_size + 2, tmp);
+    if (abort_flag) { goto Label_Abort; }
+
+    call tmp := CopyOrMoveValue(GetLocal(m, old_size + 1));
+    m := UpdateLocal(m, old_size + 6, tmp);
+    if (abort_flag) { goto Label_Abort; }
+
+    ret0 := GetLocal(m, old_size + 6);
+    return;
+    if (abort_flag) { goto Label_Abort; }
+
+Label_Abort:
+    abort_flag := true;
+    m := saved_m;
+    ret0 := DefaultValue;
+}
+
+procedure TestSpecs_div_by_zero_verify (arg0: Value, arg1: Value) returns (ret0: Value)
+{
+    call ret0 := TestSpecs_div_by_zero(arg0, arg1);
+}
+
+procedure {:inline 1} TestSpecs_div_by_zero_error (arg0: Value, arg1: Value) returns (ret0: Value)
+requires ExistsTxnSenderAccount(m, txn);
+ensures !old(b#Boolean(Boolean(true))) ==> abort_flag;
+ensures (b#Boolean(Boolean(true))) ==> !abort_flag;
+{
+    // declare local variables
+    var t0: Value; // IntegerType()
+    var t1: Value; // IntegerType()
+    var t2: Value; // IntegerType()
+    var t3: Value; // IntegerType()
+    var t4: Value; // IntegerType()
+    var t5: Value; // IntegerType()
+    var t6: Value; // IntegerType()
+
+    var tmp: Value;
+    var old_size: int;
+
+    var saved_m: Memory;
+    assume !abort_flag;
+    saved_m := m;
+
+    // assume arguments are of correct types
+    assume is#Integer(arg0);
+    assume is#Integer(arg1);
+
+    old_size := local_counter;
+    local_counter := local_counter + 7;
+    m := UpdateLocal(m, old_size + 0, arg0);
+    m := UpdateLocal(m, old_size + 1, arg1);
+
+    // bytecode translation starts here
+    call tmp := CopyOrMoveValue(GetLocal(m, old_size + 0));
+    m := UpdateLocal(m, old_size + 3, tmp);
+    if (abort_flag) { goto Label_Abort; }
+
+    call tmp := CopyOrMoveValue(GetLocal(m, old_size + 1));
+    m := UpdateLocal(m, old_size + 4, tmp);
+    if (abort_flag) { goto Label_Abort; }
+
+    call tmp := Div(GetLocal(m, old_size + 3), GetLocal(m, old_size + 4));
+    m := UpdateLocal(m, old_size + 5, tmp);
+    if (abort_flag) { goto Label_Abort; }
+
+    call tmp := CopyOrMoveValue(GetLocal(m, old_size + 5));
+    m := UpdateLocal(m, old_size + 2, tmp);
+    if (abort_flag) { goto Label_Abort; }
+
+    call tmp := CopyOrMoveValue(GetLocal(m, old_size + 1));
+    m := UpdateLocal(m, old_size + 6, tmp);
+    if (abort_flag) { goto Label_Abort; }
+
+    ret0 := GetLocal(m, old_size + 6);
+    return;
+    if (abort_flag) { goto Label_Abort; }
+
+Label_Abort:
+    abort_flag := true;
+    m := saved_m;
+    ret0 := DefaultValue;
+}
+
+procedure TestSpecs_div_by_zero_error_verify (arg0: Value, arg1: Value) returns (ret0: Value)
+{
+    call ret0 := TestSpecs_div_by_zero_error(arg0, arg1);
+}
