language/move-prover/bytecode-to-boogie/tests/goldenfiles/test3.bpl
@@ -94,7 +94,10 @@ requires ExistsTxnSenderAccount(m, txn);
 
     var tmp: Value;
     var old_size: int;
+
+    var saved_m: Memory;
     assume !abort_flag;
+    saved_m := m;
 
     // assume arguments are of correct types
     assume is#Boolean(arg0);
@@ -106,9 +109,11 @@ requires ExistsTxnSenderAccount(m, txn);
     // bytecode translation starts here
     call tmp := LdConst(0);
     m := UpdateLocal(m, old_size + 9, tmp);
+    if (abort_flag) { goto Label_Abort; }
 
     call tmp := LdConst(0);
     m := UpdateLocal(m, old_size + 10, tmp);
+    if (abort_flag) { goto Label_Abort; }
 
     assume is#Integer(GetLocal(m, old_size + 9));
 
@@ -116,202 +121,278 @@ requires ExistsTxnSenderAccount(m, txn);
 
     call tmp := Pack_Test3_T(GetLocal(m, old_size + 9), GetLocal(m, old_size + 10));
     m := UpdateLocal(m, old_size + 11, tmp);
+    if (abort_flag) { goto Label_Abort; }
 
     call tmp := CopyOrMoveValue(GetLocal(m, old_size + 11));
     m := UpdateLocal(m, old_size + 1, tmp);
+    if (abort_flag) { goto Label_Abort; }
 
     call t12 := BorrowLoc(old_size+1);
+    if (abort_flag) { goto Label_Abort; }
 
     call t2 := CopyOrMoveRef(t12);
+    if (abort_flag) { goto Label_Abort; }
 
     call tmp := CopyOrMoveValue(GetLocal(m, old_size + 0));
     m := UpdateLocal(m, old_size + 13, tmp);
+    if (abort_flag) { goto Label_Abort; }
 
     tmp := GetLocal(m, old_size + 13);
     if (!b#Boolean(tmp)) { goto Label_12; }
+    if (abort_flag) { goto Label_Abort; }
 
     call t14 := CopyOrMoveRef(t2);
+    if (abort_flag) { goto Label_Abort; }
 
     call t15 := BorrowField(t14, Test3_T_f);
+    if (abort_flag) { goto Label_Abort; }
 
     call t3 := CopyOrMoveRef(t15);
+    if (abort_flag) { goto Label_Abort; }
 
     goto Label_15;
+    if (abort_flag) { goto Label_Abort; }
 
 Label_12:
     call t16 := CopyOrMoveRef(t2);
+    if (abort_flag) { goto Label_Abort; }
 
     call t17 := BorrowField(t16, Test3_T_g);
+    if (abort_flag) { goto Label_Abort; }
 
     call t3 := CopyOrMoveRef(t17);
+    if (abort_flag) { goto Label_Abort; }
 
 Label_15:
     call tmp := LdConst(10);
     m := UpdateLocal(m, old_size + 18, tmp);
+    if (abort_flag) { goto Label_Abort; }
 
     call t19 := CopyOrMoveRef(t3);
+    if (abort_flag) { goto Label_Abort; }
 
     call WriteRef(t19, GetLocal(m, old_size + 18));
+    if (abort_flag) { goto Label_Abort; }
 
     call tmp := CopyOrMoveValue(GetLocal(m, old_size + 0));
     m := UpdateLocal(m, old_size + 20, tmp);
+    if (abort_flag) { goto Label_Abort; }
 
     call tmp := Not(GetLocal(m, old_size + 20));
     m := UpdateLocal(m, old_size + 21, tmp);
+    if (abort_flag) { goto Label_Abort; }
 
     tmp := GetLocal(m, old_size + 21);
     if (!b#Boolean(tmp)) { goto Label_25; }
+    if (abort_flag) { goto Label_Abort; }
 
     call t22 := CopyOrMoveRef(t2);
+    if (abort_flag) { goto Label_Abort; }
 
     call t23 := BorrowField(t22, Test3_T_f);
+    if (abort_flag) { goto Label_Abort; }
 
     call t4 := CopyOrMoveRef(t23);
+    if (abort_flag) { goto Label_Abort; }
 
     goto Label_28;
+    if (abort_flag) { goto Label_Abort; }
 
 Label_25:
     call t24 := CopyOrMoveRef(t2);
+    if (abort_flag) { goto Label_Abort; }
 
     call t25 := BorrowField(t24, Test3_T_g);
+    if (abort_flag) { goto Label_Abort; }
 
     call t4 := CopyOrMoveRef(t25);
+    if (abort_flag) { goto Label_Abort; }
 
 Label_28:
     call tmp := LdConst(20);
     m := UpdateLocal(m, old_size + 26, tmp);
+    if (abort_flag) { goto Label_Abort; }
 
     call t27 := CopyOrMoveRef(t4);
+    if (abort_flag) { goto Label_Abort; }
 
     call WriteRef(t27, GetLocal(m, old_size + 26));
+    if (abort_flag) { goto Label_Abort; }
 
     call t28 := CopyOrMoveRef(t2);
+    if (abort_flag) { goto Label_Abort; }
 
     call t29 := BorrowField(t28, Test3_T_f);
+    if (abort_flag) { goto Label_Abort; }
 
     call t5 := CopyOrMoveRef(t29);
+    if (abort_flag) { goto Label_Abort; }
 
     call t30 := CopyOrMoveRef(t2);
+    if (abort_flag) { goto Label_Abort; }
 
     call t31 := BorrowField(t30, Test3_T_g);
+    if (abort_flag) { goto Label_Abort; }
 
     call t6 := CopyOrMoveRef(t31);
+    if (abort_flag) { goto Label_Abort; }
 
     call t32 := CopyOrMoveRef(t5);
+    if (abort_flag) { goto Label_Abort; }
 
     call tmp := ReadRef(t32);
     assume is#Integer(tmp);
 
     m := UpdateLocal(m, old_size + 33, tmp);
+    if (abort_flag) { goto Label_Abort; }
 
     call tmp := CopyOrMoveValue(GetLocal(m, old_size + 33));
     m := UpdateLocal(m, old_size + 7, tmp);
+    if (abort_flag) { goto Label_Abort; }
 
     call t34 := CopyOrMoveRef(t6);
+    if (abort_flag) { goto Label_Abort; }
 
     call tmp := ReadRef(t34);
     assume is#Integer(tmp);
 
     m := UpdateLocal(m, old_size + 35, tmp);
+    if (abort_flag) { goto Label_Abort; }
 
     call tmp := CopyOrMoveValue(GetLocal(m, old_size + 35));
     m := UpdateLocal(m, old_size + 8, tmp);
+    if (abort_flag) { goto Label_Abort; }
 
     call tmp := CopyOrMoveValue(GetLocal(m, old_size + 0));
     m := UpdateLocal(m, old_size + 36, tmp);
+    if (abort_flag) { goto Label_Abort; }
 
     tmp := GetLocal(m, old_size + 36);
     if (!b#Boolean(tmp)) { goto Label_60; }
+    if (abort_flag) { goto Label_Abort; }
 
     call tmp := CopyOrMoveValue(GetLocal(m, old_size + 7));
     m := UpdateLocal(m, old_size + 37, tmp);
+    if (abort_flag) { goto Label_Abort; }
 
     call tmp := LdConst(10);
     m := UpdateLocal(m, old_size + 38, tmp);
+    if (abort_flag) { goto Label_Abort; }
 
     tmp := Boolean(IsEqual(GetLocal(m, old_size + 37), GetLocal(m, old_size + 38)));
     m := UpdateLocal(m, old_size + 39, tmp);
+    if (abort_flag) { goto Label_Abort; }
 
     call tmp := Not(GetLocal(m, old_size + 39));
     m := UpdateLocal(m, old_size + 40, tmp);
+    if (abort_flag) { goto Label_Abort; }
 
     tmp := GetLocal(m, old_size + 40);
     if (!b#Boolean(tmp)) { goto Label_52; }
+    if (abort_flag) { goto Label_Abort; }
 
     call tmp := LdConst(42);
     m := UpdateLocal(m, old_size + 41, tmp);
+    if (abort_flag) { goto Label_Abort; }
 
-    assert false;
+    goto Label_Abort;
+    if (abort_flag) { goto Label_Abort; }
 
 Label_52:
     call tmp := CopyOrMoveValue(GetLocal(m, old_size + 8));
     m := UpdateLocal(m, old_size + 42, tmp);
+    if (abort_flag) { goto Label_Abort; }
 
     call tmp := LdConst(20);
     m := UpdateLocal(m, old_size + 43, tmp);
+    if (abort_flag) { goto Label_Abort; }
 
     tmp := Boolean(IsEqual(GetLocal(m, old_size + 42), GetLocal(m, old_size + 43)));
     m := UpdateLocal(m, old_size + 44, tmp);
+    if (abort_flag) { goto Label_Abort; }
 
     call tmp := Not(GetLocal(m, old_size + 44));
     m := UpdateLocal(m, old_size + 45, tmp);
+    if (abort_flag) { goto Label_Abort; }
 
     tmp := GetLocal(m, old_size + 45);
     if (!b#Boolean(tmp)) { goto Label_59; }
+    if (abort_flag) { goto Label_Abort; }
 
     call tmp := LdConst(42);
     m := UpdateLocal(m, old_size + 46, tmp);
+    if (abort_flag) { goto Label_Abort; }
 
-    assert false;
+    goto Label_Abort;
+    if (abort_flag) { goto Label_Abort; }
 
 Label_59:
     goto Label_74;
+    if (abort_flag) { goto Label_Abort; }
 
 Label_60:
     call tmp := CopyOrMoveValue(GetLocal(m, old_size + 7));
     m := UpdateLocal(m, old_size + 47, tmp);
+    if (abort_flag) { goto Label_Abort; }
 
     call tmp := LdConst(20);
     m := UpdateLocal(m, old_size + 48, tmp);
+    if (abort_flag) { goto Label_Abort; }
 
     tmp := Boolean(IsEqual(GetLocal(m, old_size + 47), GetLocal(m, old_size + 48)));
     m := UpdateLocal(m, old_size + 49, tmp);
+    if (abort_flag) { goto Label_Abort; }
 
     call tmp := Not(GetLocal(m, old_size + 49));
     m := UpdateLocal(m, old_size + 50, tmp);
+    if (abort_flag) { goto Label_Abort; }
 
     tmp := GetLocal(m, old_size + 50);
     if (!b#Boolean(tmp)) { goto Label_67; }
+    if (abort_flag) { goto Label_Abort; }
 
     call tmp := LdConst(42);
     m := UpdateLocal(m, old_size + 51, tmp);
+    if (abort_flag) { goto Label_Abort; }
 
-    assert false;
+    goto Label_Abort;
+    if (abort_flag) { goto Label_Abort; }
 
 Label_67:
     call tmp := CopyOrMoveValue(GetLocal(m, old_size + 8));
     m := UpdateLocal(m, old_size + 52, tmp);
+    if (abort_flag) { goto Label_Abort; }
 
     call tmp := LdConst(10);
     m := UpdateLocal(m, old_size + 53, tmp);
+    if (abort_flag) { goto Label_Abort; }
 
     tmp := Boolean(IsEqual(GetLocal(m, old_size + 52), GetLocal(m, old_size + 53)));
     m := UpdateLocal(m, old_size + 54, tmp);
+    if (abort_flag) { goto Label_Abort; }
 
     call tmp := Not(GetLocal(m, old_size + 54));
     m := UpdateLocal(m, old_size + 55, tmp);
+    if (abort_flag) { goto Label_Abort; }
 
     tmp := GetLocal(m, old_size + 55);
     if (!b#Boolean(tmp)) { goto Label_74; }
+    if (abort_flag) { goto Label_Abort; }
 
     call tmp := LdConst(42);
     m := UpdateLocal(m, old_size + 56, tmp);
+    if (abort_flag) { goto Label_Abort; }
 
-    assert false;
+    goto Label_Abort;
+    if (abort_flag) { goto Label_Abort; }
 
 Label_74:
     return;
+    if (abort_flag) { goto Label_Abort; }
 
+Label_Abort:
+    abort_flag := true;
+    m := saved_m;
 }
 
 procedure Test3_test3_verify (arg0: Value) returns ()
